Prove cases 1 and 2 for 'segment_length_lb'
That is, prove that the lower bound on segment length holds for
segments of length 1, and follows from induction for segments that
begin with a forward step. I expect there to be 6 cases in-total.
Here are the other four:
 3) Segment begins with a right turn
 4) Segment begins with a left turn and contains no other turns
 5) Segment begins with a left turn, moves straight for some number
    of steps, and then turns left again
 6) Segment begins with a left turn, moves straight for some number
    of steps, and then turns right

This change also includes some useful identities relating the start
and end of split segments to the original segment and to each-other.
It also includes proofs for the lengths of split segments.

AngelDevil/Segment.lean
@@ -17,6 +17,10 @@ set_option linter.style.longLine false
 def manhattan (a b : Int × Int) : Nat :=
   Int.natAbs (b.1 - a.1) + Int.natAbs (b.2 - a.2)
 
+lemma manhattan_self (a : Int × Int) :
+  manhattan a a = 0 := by
+  unfold manhattan; simp
+
 -- The triangular inequality for Manhattan distance
 lemma manhattan_tri (a b c : Int × Int) :
   manhattan a c ≤ manhattan a b + manhattan b c := by
@@ -78,6 +82,11 @@ def segment_split_second (seg : TraceSegment) (k : Nat) (_ : seg.i ≤ k) (kle :
   ile := kle
   jlt := seg.jlt
 
+lemma segment_length_pos (seg : TraceSegment) :
+  0 < segment_length seg := by
+  unfold segment_length
+  exact Nat.add_one_pos _
+
 -- The length of the segment states is the same as the segment length
 lemma segment_states_length (seg : TraceSegment) :
   (segment_states seg).length = (segment_length seg) := by
@@ -86,6 +95,36 @@ lemma segment_states_length (seg : TraceSegment) :
   rw [List.length_drop, trace_length]
   apply Nat.add_one_le_of_lt (Nat.sub_lt_sub_right seg.ile _)
   apply (trace_length _ _ _) ▸ seg.jlt
+
+lemma segment_start_eq_getElem_zero (seg : TraceSegment) :
+  segment_start seg = (segment_states seg)[0]'(by
+    rw [segment_states_length, segment_length]
+    exact Nat.add_one_pos _
+  ) := by
+  unfold segment_start segment_states
+  rw [List.getElem_take, List.getElem_drop]
+  rw [getElem_congr_idx (Nat.add_zero _)]
+
+lemma segment_end_eq_getElem (seg : TraceSegment) :
+  segment_end seg = (segment_states seg)[segment_length seg - 1]'(by
+    rw [segment_states_length]
+    apply Nat.sub_one_lt (Nat.ne_zero_of_lt (segment_length_pos seg))
+  ) := by
+  unfold segment_end segment_states
+  rw [List.getElem_take, List.getElem_drop]; congr
+  rw [segment_length, Nat.add_one_sub_one]
+  apply (Nat.add_sub_cancel' _).symm
+  exact seg.ile
+
+lemma segment_split_first_start (seg : TraceSegment) (k : Nat) (lek : seg.i ≤ k) (kle : k ≤ seg.j) :
+  segment_start (segment_split_first seg k lek kle) = segment_start seg := rfl
+
+lemma segment_split_second_end (seg : TraceSegment) (k : Nat) (lek : seg.i ≤ k) (kle : k ≤ seg.j) :
+  segment_end (segment_split_second seg k lek kle) = segment_end seg := rfl
+
+lemma segment_split_overlap (seg : TraceSegment) (k : Nat) (lek : seg.i ≤ k) (kle : k ≤ seg.j) :
+  segment_end (segment_split_first seg k lek kle) =
+  segment_start (segment_split_second seg k lek kle) := rfl
 
 -- Get the length of the first half of a split trace
 lemma segment_split_first_length (seg : TraceSegment) (k : Nat) (lek : seg.i ≤ k) (kle : k ≤ seg.j) :
@@ -194,3 +233,71 @@ lemma segment_split_states (seg : TraceSegment) (k : Nat) (lek : seg.i ≤ k) (k
       exact le_of_lt (lt_of_le_of_lt lek (Nat.lt_add_one _))
     rw [Nat.sub_add_comm lek, Nat.sub_add_cancel]
     rwa [segment_states_length, segment_split_first_length] at lea
+
+-- Check if the 'move' between state 'a' and state 'a+1' is 'f'
+def check_for_move (seg : TraceSegment)
+  (f : RunState → RunState) (a : Nat) (alt : a + 1 < segment_length seg) : Prop :=
+  f ((segment_states seg)[a]'(by
+    rw [segment_states_length]
+    exact lt_trans (Nat.lt_add_one _) alt
+  )) = (segment_states seg)[a + 1]'(by rwa [segment_states_length])
+
+def segment_starts_with_move_forward (seg : TraceSegment) (h : 1 < segment_length seg) : Prop :=
+  check_for_move seg move_forward 0 h
+
+def segment_length_lb_prop (seg : TraceSegment) : Prop :=
+  manhattan (loc (segment_start seg)) (loc (segment_end seg)) ≤ segment_length seg
+
+-- Prove the segment length lower bound when the length is 1
+lemma segment_length_lb_case1 (seg : TraceSegment) (h : segment_length seg = 1) :
+  segment_length_lb_prop seg := by
+  unfold segment_length_lb_prop
+  unfold segment_length at h
+  -- If length = 1, i = j
+  have hij := le_antisymm seg.ile (Nat.le_of_sub_eq_zero (Nat.add_right_cancel h))
+  convert Nat.zero_le _
+  convert manhattan_self _ using 2
+  unfold segment_start segment_end
+  rw [getElem_congr_idx hij]
+
+-- Prove the induction case for the length lower bound when
+-- the segment begins with a 'move forward'
+lemma segment_length_lb_case2 (seg : TraceSegment) (h : 1 < segment_length seg) :
+  segment_starts_with_move_forward seg h →
+  segment_length_lb_prop (segment_split_second seg (seg.i + 1) (Nat.le_add_right _ _)
+    (Nat.add_one_le_of_lt (Nat.lt_of_sub_pos (Nat.pos_of_lt_add_left h)))) →
+  segment_length_lb_prop seg := by
+  unfold segment_length_lb_prop
+  intro hmf hllb
+  let k := seg.i + 1
+  have lek : seg.i ≤ k := Nat.le_add_right _ _
+  have kle : k ≤ seg.j :=
+    Nat.add_one_le_of_lt (Nat.lt_of_sub_pos (Nat.pos_of_lt_add_left h))
+  rw [segment_split_length seg k lek kle]
+  rw [segment_split_first_length]
+  rw [Nat.sub_add_comm (Nat.le_refl seg.i), Nat.sub_self, zero_add]
+  rw [add_right_comm, Nat.add_one_sub_one, add_comm]
+  let seg_first := segment_split_first seg k lek kle
+  let seg_second := segment_split_second seg k lek kle
+  apply le_trans (manhattan_tri _ _ _)
+  change manhattan _ (loc (segment_start seg_second)) + _ ≤ _
+  rw [← segment_split_first_start seg k lek kle]
+  rw [← segment_split_second_end seg k lek kle]
+  nth_rw 1 [← segment_split_overlap]
+  rw [add_comm]
+  convert Nat.add_le_add_right hllb 1
+  unfold segment_starts_with_move_forward check_for_move at hmf
+  rw [← segment_start_eq_getElem_zero, getElem_congr_idx (Nat.zero_add _)] at hmf
+  rw [← segment_split_first_start seg k lek kle] at hmf
+  have : segment_end seg_first = (segment_states seg)[1]'(by rwa [segment_states_length]) := by
+    rw [segment_end_eq_getElem, getElem_congr_coll (segment_split_first_states _ _ _ _)]
+    rw [List.getElem_take]; congr
+    rw [segment_split_first_length, Nat.add_one_sub_one]
+    unfold k
+    rw [add_comm, Nat.add_sub_cancel]
+  rw [← this] at hmf
+  rw [← hmf]
+  let s := segment_start seg_first
+  change manhattan (loc s) (loc (move_forward s)) = 1
+  unfold manhattan move_forward loc; simp
+  exact uvec_xabs_add_yabs_eq_one _
